rnm checkpoint

theories/diffpriv/examples/report_noisy_max.v
@@ -1,34 +1,52 @@
+From iris.base_logic Require Export na_invariants.
 From clutch.common Require Import inject.
+From clutch.prelude Require Import tactics.
 From clutch.prob Require Import differential_privacy.
 From clutch.diffpriv Require Import adequacy diffpriv proofmode.
 
+Definition logN : namespace := nroot .@ "logN".
+
+Class diffprivRGS Σ := DiffprivRGS {
+                           diffprivRGS_diffprivGS :: diffprivGS Σ;
+                           diffprivRGS_na_invG :: na_invG Σ;
+                           diffprivRGS_nais : na_inv_pool_name;
+                         }.
+
+Definition na_ownP `{!diffprivRGS Σ} := na_own diffprivRGS_nais.
+Definition na_invP `{!diffprivRGS Σ} := na_inv diffprivRGS_nais.
+Definition na_closeP `{!diffprivRGS Σ} P N E := (▷ P ∗ na_ownP (E ∖ ↑N) ={⊤}=∗ na_ownP E)%I.
+
+
 Section rnm.
-  Context `{!diffprivGS Σ}.
+  Context `{!diffprivRGS Σ}.
 
   #[local] Open Scope R.
 
   Definition report_noisy_max (num den : Z) : val :=
     λ:"evalQ" "N" "d",
-      let: "maxI" := ref #(-1) in
+      let: "maxI" := ref #(0) in
       let: "maxA" := ref #0 in
+      let: "cur" := ref #0 in
       let: "f" :=
         (rec: "rnm" "i" :=
          if: "i" = "N" then
            ! "maxI"
          else
-           (let: "a" := Laplace #num #(2 * den) ("evalQ" "i" "d") in
-           (if: (! "maxI" = #(-1)) `or` (! "maxA" < "a") then
+           (let: "a" := Laplace #num #(den) ("evalQ" "i" "d") in
+            "cur" <- "a" ;;
+           (if: (* (! "maxI" = #(-1)) `or` *) (! "maxA" < "a") then
              "maxA" <- "a" ;;
              "maxI" <- "i"
            else #()) ;;
            "rnm" ("i" + #1)))
       in "f" #0.
 
-  Definition rnm_body (num den : Z) (evalQ : val) {DB} (dDB : Distance DB) (N : nat) (db : DB) (maxI maxA : loc) :=
+  Definition rnm_body (num den : Z) (evalQ : val) {DB} (dDB : Distance DB) (N : nat) (db : DB) (maxI maxA cur : loc) :=
     (rec: "rnm" "i" :=
         if: "i" = #N then ! #maxI
-        else let: "a" := Laplace #num #(2 * den) (evalQ "i" (inject db)) in
-             (if: ! #maxI = #0 `or` ! #maxA < "a"
+        else let: "a" := Laplace #num #(den) (evalQ "i" (inject db)) in
+            #cur <- "a" ;;
+             (if: (* ! #maxI = #(-1) `or` *) ! #maxA < "a"
               then #maxA <- "a";; #maxI <- "i" else #());;
              "rnm" ("i" + #1))%V.
 
@@ -71,6 +89,415 @@ Section rnm.
     λ:"i" "db", if: "i" = #0 then count_under_40 "db"
                else if: "i" = #1 then count_over_80 "db"
                     else #0.
+
+  (* Definition rwp (e e' : expr) E (R : val → val → iProp Σ) : iProp Σ :=
+       (⤇ e' -∗ WP e @ E {{ v, ∃ v', R v v' }})%I.
+
+     (* Notation "'RWP' e ~ e' {{ Φ } } " := (rwp e e' top Φ) (only parsing).
+        Notation "'RWP' e ~ e' @ E {{ Φ } } " := (rwp e e' E Φ) (only parsing). *)
+     (* Notation "'RWP' e ~ e' @ E {{ v v' , Φ } } " := (rwp e e' E (λ v v', Φ)). *)
+
+     Notation "'RWP' e << e' {{ v , v' , Φ } } " := (rwp e e' top (λ v v', Φ))
+       (at level 20, e, e', Φ at level 200,
+      format "'[hv' 'RWP'  e  <<  e'  '/' {{  '[' v ,  v' ,  Φ  ']' } } ']'") : bi_scope.
+
+     Lemma pweq (e e' : expr) :
+       (⊢ RWP e << e' {{ v , v' ,  ⌜ v = v' ⌝ }})
+       →
+       (∀ x : val, ⤇ e' ⊢ WP e {{ v, ∃ v', ⤇ (of_val v') ∗ ⌜v = x -> v' = x⌝}})
+       →
+         (⤇ e' ⊢ WP e {{ v, ∃ v', ⤇ (of_val v') ∗ ⌜v = v'⌝ }}). *)
+
+  Lemma pweq_weak (e e' : expr) K :
+    (⊢ (⤇ e' -∗ WP e {{ v, ∃ v', ⤇ (of_val v')}}))
+    →
+    (⤇ fill K e' -∗ WP e {{ v, (∃ z : Z, ⌜v = #z⌝)
+                               ∗ ∃ v', ⤇ fill K (of_val v') ∗ ⌜∀ x : Z, v = #x -> v' = #x⌝}})
+    -∗
+      (⤇ fill K e' -∗ WP e {{ v, ∃ z : Z, ⌜v = #z⌝ ∗ ⤇ fill K (of_val v) }}).
+  Proof.
+    iIntros (?) "h Ke'".
+    iSpecialize ("h" with "Ke'").
+    iApply (wp_mono with "h").
+    iIntros (v) "((%z & %eq_v_z) & %v' & Kv' & %alleq)".
+    iExists z. rewrite (alleq _ eq_v_z). rewrite eq_v_z. iFrame. done.
+  Qed.
+
+
+  (* Lemma pweq (e e' : expr) K :
+       (* (⊢ (⤇ e' -∗ WP e {{ v, ∃ v', ⤇ (of_val v')}}))
+          → *)
+       ∀ x : Z,
+       ( ⤇ fill K e' -∗ WP e {{ v, ∃ v', ⤇ fill K (of_val v') ∗ ⌜v = #x -> v' = #x⌝}})
+       -∗
+         (⤇ fill K e' -∗ WP e {{ v, ∃ z : Z, ⌜v = #z⌝ ∗ ⤇ fill K (of_val v) }}).
+     (* Admitted. *)
+     Proof.
+       intros x. iIntros "alleq e'".
+       (* iDestruct (safe with "[$e']") as "H". *)
+       iDestruct ("alleq" with "[$e']") as "H".
+       iApply (wp_mono with "H").
+       iIntros (v) "(%v' & v' & %h)".
+       iExists _.
+       rewrite h.
+       iSplitR ; [iPureIntro|]. *)
+Lemma pweq (e e' : expr) K :
+  (∀ x : Z, ⤇ fill K e' -∗ WP e {{ v, ∃ v', ⤇ fill K (of_val v') ∗ ⌜v = #x -> v' = #x⌝}})
+  -∗
+  ({{{ ⤇ fill K e'}}} e {{{ (v : Z), RET #v; ⤇ fill K (of_val #v) }}}).
+Admitted.
+
+
+  Lemma rnm_pw_diffpriv num den (evalQ : val) DB (dDB : Distance DB) (N : nat) K :
+    (0 < IZR num / IZR den) →
+    (∀ i : Z, wp_sensitive (evalQ #i) 1 dDB dZ) →
+    ∀ db db', dDB db db' <= 1 →
+              ∀ j : Z,
+                {{{ ↯ (IZR num / IZR den) ∗
+                    ⤇ fill K (report_noisy_max num den evalQ #N (inject db')) }}}
+                  report_noisy_max num den evalQ #N (inject db)
+                  {{{ v, RET v ; ∃ v', ⤇ fill K v' ∗ ⌜ v = #j → v' = #j ⌝  }}}
+  .
+  Proof with (tp_pures ; wp_pures).
+    intros εpos qi_sens.
+    iIntros (db db' db_adj x Φ) "(ε & rnm) HΦ".
+    rewrite /report_noisy_max.
+    simpl.
+    tp_pures.
+    wp_pures.
+    tp_alloc as maxI2 "maxI2". tp_pures. tp_alloc as maxA2 "maxA2". tp_pures. tp_alloc as cur2 "cur2".  do 5 tp_pure.
+    wp_pures. wp_alloc maxI1 as "maxI1". wp_alloc maxA1 as "maxA1". wp_alloc cur1 as "cur1".  do 5 wp_pure.
+    rewrite -/(rnm_body num den evalQ dDB N db maxI1 maxA1 cur1).
+    rewrite -/(rnm_body num den evalQ dDB N db' maxI2 maxA2 cur2).
+    rename x into j.
+    cut
+      (∀ (i imax1 imax2 : Z) (amax1 amax2 vcur1 vcur2 : Z),
+          {{{ maxI1 ↦ #imax1 ∗ maxI2 ↦ₛ #imax2 ∗ maxA1 ↦ #amax1 ∗ maxA2 ↦ₛ #amax2
+              ∗ cur1 ↦ #vcur1 ∗ cur2 ↦ₛ #vcur2
+              ∗ ↯ (if (bool_decide (i <= j))%Z then (IZR num / IZR den) else 0)
+              ∗ ⤇ fill K (rnm_body num den evalQ dDB N db' maxI2 maxA2 cur2 #i)
+              ∗ ⌜ i < j
+                  → ((dZ amax1 amax2 <= 1)%R
+                     ∧ imax1 < i ∧ imax2 < i
+                     ∧ (¬ (i <= N ∧ i < j) → i = j)) ⌝%Z
+              ∗ ⌜ i = j
+                  → ( (dZ amax1 amax2 <= 1)%R
+                      ∧ (imax1 = j → (imax2 = j ∧ amax1 + 1 = amax2))
+                      ∧ (¬ (i <= N ∧ i = j) → i = j+1) )%Z ⌝
+              ∗ ⌜ (j < i)%Z
+                  → ( imax1 = j → (imax2 = j ∧ amax1 + 1 = amax2) )%Z ⌝
+          }}}
+            rnm_body num den evalQ dDB N db maxI1 maxA1 cur1 #i
+            {{{ (v : Z), RET #v;
+                ∃ (v' : Z), ⤇ fill K #v' ∗ ⌜ v = j -> v' = j ⌝
+            }}}
+      ).
+    1: { intros h.
+         iMod ec_zero as "ε0".
+         iApply (h with "[-HΦ]").
+         - (* We have all the reference resources for the IH. *)
+           iFrame.
+           iSplitL.
+           (* We have the error credits too *)
+           + case_bool_decide ; iFrame.
+           (* and the arithmetic works out fine *)
+           + iPureIntro. split ; [|split].
+             * clear. intros. repeat split.
+               -- rewrite distance_0 ; lra.
+               -- give_up.
+               -- give_up.
+               -- intros []. lia.
+             * clear. intros. repeat split. all: try lia.
+               -- rewrite distance_0 ; lra.
+               -- subst. give_up.
+             * clear. intros. exfalso. lia.
+         - (* The post-condition of the IH implies the original post. *)
+           iNext ; iIntros (v) "(%v' & v' & %h')".
+           iApply "HΦ". iExists _. iFrame.
+           iPureIntro. intro h''. do 3 f_equal. apply h'. inversion h''. done.
+    }
+    clear Φ.
+    iLöb as "IH".
+    iIntros (j i imax1 imax2 amax1 amax2 vcur1 vcur2 Φ) "(maxI1 & maxI2 & maxA1 & maxA2 & cur1 & cur2 & ε & rnm' & %maxcur1 & %maxcur2 & %imax12 & %iN) HΦ".
+    rewrite {4}/rnm_body. wp_pures.
+    rewrite {3}/rnm_body. tp_pures ; [cbv ; auto|].
+    case_bool_decide (#i = #N).
+    - tp_pures. wp_pures. tp_load ; wp_load. iApply "HΦ". iExists imax2. iFrame "rnm'". iPureIntro.
+      intros ij1. inversion H.
+      try lia.
+    - tp_pures ; wp_pures.
+    rewrite -/(rnm_body _ _ _ _ _ _ _ maxA1 _).
+    rewrite -/(rnm_body _ _ _ _ _ _ _ maxA2 _).
+    tp_bind (evalQ _ _).
+    wp_bind (evalQ _ _).
+    iAssert ({{{⌜True⌝}}} evalQ #i (inject db) {{{ v, RET v; ∃ z : Z, ⌜v = #z⌝ }}})%I as "wp_ev". 1: admit.
+    iApply "wp_ev" => // ; iIntros "!> % [%e1 ->]" ; iClear "wp_ev".
+    iAssert (∀ K, ⤇ fill K (evalQ #i (inject db')) -∗ spec_update top (∃ z : Z, ⤇ fill K #z))%I as "tp_ev". 1: admit.
+    iMod ("tp_ev" with "rnm'") as "[%e2 rnm']" => /= ; iClear "tp_ev".
+    destruct (make_decision (i = j)) as [e|n].
+
+
+  Lemma rnm_diffpriv num den (evalQ : val) DB (dDB : Distance DB) (N : nat) :
+    (0 < IZR num / IZR den) →
+    (∀ i : Z, wp_sensitive (evalQ #i) 1 dDB dZ) →
+    wp_diffpriv (report_noisy_max num den evalQ #N) (IZR num / IZR den) dDB.
+  Proof with (tp_pures ; wp_pures).
+    intros εpos qi_sens.
+    iIntros (? c db db' db_adj Φ) "(rnm & ε) HΦ".
+    rewrite /report_noisy_max.
+    tp_pures.
+    tp_alloc as maxI2 "maxI2". tp_pures. tp_alloc as maxA2 "maxA2". tp_pures. tp_alloc as cur2 "cur2".  do 5 tp_pure.
+    wp_pures. wp_alloc maxI1 as "maxI1". wp_alloc maxA1 as "maxA1". wp_alloc cur1 as "cur1".  do 5 wp_pure.
+    rewrite -/(rnm_body num den evalQ dDB N db maxI1 maxA1 cur1).
+    rewrite -/(rnm_body num den evalQ dDB N db' maxI2 maxA2 cur2).
+    iApply (pweq with "[-HΦ rnm] [$rnm] [HΦ]"). 2: iNext ; iIntros ; iApply "HΦ" ; done.
+    clear Φ.
+    iIntros (x) "rnm'".
+
+    cut
+      (∀ (j i imax1 imax2 : Z) (amax1 amax2 vcur1 vcur2 : Z),
+          {{{ maxI1 ↦ #imax1 ∗ maxI2 ↦ₛ #imax2 ∗ maxA1 ↦ #amax1 ∗ maxA2 ↦ₛ #amax2
+              ∗ cur1 ↦ #vcur1 ∗ cur2 ↦ₛ #vcur2
+              ∗ ↯ (if (bool_decide (i <= j))%Z then c * (IZR num / IZR den) else 0)
+              ∗ ⤇ fill K (rnm_body num den evalQ dDB N db' maxI2 maxA2 cur2 #i)
+              ∗ ⌜(amax1 < vcur1 → imax1 = i)%Z⌝
+              ∗ ⌜(amax2 < vcur2 → imax1 = i)%Z⌝
+              ∗ ⌜ imax1 = imax2 ⌝
+              (* ∗ ⌜((i = N → imax1 = j → imax2 = j))%Z⌝ *)
+              ∗ ⌜True%Z⌝
+          }}}
+            rnm_body num den evalQ dDB N db maxI1 maxA1 cur1 #i
+            {{{ (v : Z), RET #v;
+                ∃ (v' : Z), ⤇ fill K #v' ∗ ⌜ v = j -> v' = j ⌝
+            }}}
+
+      ).
+
+    1: { intros h.
+         iMod ec_zero as "ε0".
+         iApply (h x with "[-]").
+         - (* We have all the reference resources for the IH. *)
+           iFrame.
+           iSplitL.
+           (* We have the error credits too *)
+           + case_bool_decide ; iFrame.
+           (* and the arithmetic works out fine *)
+           + iPureIntro. repeat split. all: auto.
+         - (* The post-condition of the IH implies the original post. *)
+           iNext ; iIntros (v) "(%v' & v' & %h')".
+           iExists _. iFrame.
+           iPureIntro. intro h''. do 2 f_equal. apply h'. inversion h''. done.
+    }
+    iLöb as "IH".
+    iIntros (j i imax1 imax2 amax1 amax2 vcur1 vcur2 Φ) "(maxI1 & maxI2 & maxA1 & maxA2 & cur1 & cur2 & ε & rnm' & %maxcur1 & %maxcur2 & %imax12 & %iN) HΦ".
+    rewrite {4}/rnm_body. wp_pures.
+    rewrite {3}/rnm_body. tp_pures ; [cbv ; auto|].
+    case_bool_decide (#i = #N).
+    - tp_pures. wp_pures. tp_load ; wp_load. iApply "HΦ". iExists imax2. iFrame "rnm'". iPureIntro.
+      intros ij1. inversion H.
+      try lia.
+    - tp_pures ; wp_pures.
+    rewrite -/(rnm_body _ _ _ _ _ _ _ maxA1 _).
+    rewrite -/(rnm_body _ _ _ _ _ _ _ maxA2 _).
+    tp_bind (evalQ _ _).
+    wp_bind (evalQ _ _).
+    iAssert ({{{⌜True⌝}}} evalQ #i (inject db) {{{ v, RET v; ∃ z : Z, ⌜v = #z⌝ }}})%I as "wp_ev". 1: admit.
+    iApply "wp_ev" => // ; iIntros "!> % [%e1 ->]" ; iClear "wp_ev".
+    iAssert (∀ K, ⤇ fill K (evalQ #i (inject db')) -∗ spec_update top (∃ z : Z, ⤇ fill K #z))%I as "tp_ev". 1: admit.
+    iMod ("tp_ev" with "rnm'") as "[%e2 rnm']" => /= ; iClear "tp_ev".
+    destruct (make_decision (i = j)) as [e|n].
+    + tp_bind (Laplace _ _ _).
+      wp_bind (Laplace _ _ _).
+      (* the Laplace sampling should preserve the two assumptions that
+           if (the value stored at maxA1) < (the value stored at cur1)
+           then (the val stored at maxI1) = i
+         and
+           if (the value stored at maxA2) < (the value stored at cur2)
+           then (the val stored at maxI1) = i
+         i.e., preserve
+  maxcur1 : (amax1 < vcur1)%Z → imax1 = i
+  maxcur2 : (amax2 < vcur2)%Z → imax1 = i
+         where vcur1 and vcur2 are updated to be `a`, the result of the sampling
+       *)
+      iApply (wp_couple_laplace e1 e2 0%Z 1%Z with "[$rnm' ε]") => //.
+      {
+        (* sensitivity of evalQ *)
+        admit.
+      }
+      { case_bool_decide. 2: lia.
+        (* would be fine if we had phrased the adjacency of db and db' as dDB db db' <= 1. *)
+        admit.
+      }
+      iNext ; iIntros (a) "rnm'" => /=.
+      wp_pures. tp_pures. rewrite !Zplus_0_r.
+      tp_store ; tp_pures ; wp_store.
+      (* both samplings resolve to the same `a`, so the implications above become... *)
+      assert (amax1 < a → imax1 = i)%Z as amax1_i.
+      {
+        intros.
+      }
+      assert (amax2 < a → imax1 = i)%Z as amax2_i by admit.
+      tp_load ; wp_load ; tp_pures ; wp_pures.
+      case_bool_decide (amax1 < a)%Z as case_l ; tp_pures ; wp_pures.
+      all: case_bool_decide as case_r ; tp_pures ; wp_pures.
+      * do 2 (tp_store ; tp_pures ; wp_store ; wp_pures).
+        iMod ec_zero as "ε0".
+        iApply ("IH" $! j with "[-HΦ]") ; iFrame.
+        rewrite e. case_bool_decide ; try lia. iFrame.
+        iPureIntro. intuition lia.
+      * iMod ec_zero as "ε0".
+        wp_store ; wp_pures ; wp_store ; wp_pures.
+        iSpecialize ("IH" $! j (i+1)%Z i imax2 a amax2 a a).
+        iSpecialize ("IH" with "[ε0 $rnm' $maxA1 $maxA2 $maxI1 $maxI2 $cur1 $cur2]").
+        2: iApply ("IH" with "[HΦ]") ; iFrame.
+        iSplitL. 1: case_bool_decide ; try lia ; iFrame "ε0".
+        iPureIntro ; split ; [|split ; [|split]].
+        1,2,4: intuition lia.
+
+        (* to show: the outputs are equal. we updated the left but not the right. *)
+
+assert
+(forall DB (adj : DB → DB → Prop) db1 db2 i1 i2 output1 output2 max1 max2 cur1 cur2 N k,
+  (((adj db1 db2 /\
+    i1 = i2 /\
+    output1 = output2 /\
+    (max1 < cur1 ->
+     output1 = i1) /\
+    (max2 < cur2 ->
+     output1 = i1) /\
+    i1 < N /\
+    k = N - i1 - 1 /\
+    N - i1 - 1 <= N /\
+    cur1 = cur2) /\
+   max1 < cur1) /\
+   (¬ (max2 < cur2))) ->
+  (let max_L := cur1 in
+   let output_L := i1 in
+   let i_R := i2 + 1 in
+   let i_L := i1 + 1 in
+  (adj db1 db2 /\
+   (i_L = i_R /\ output_L = output2) /\
+   (max_L < cur1 -> output_L = i_L) /\
+   (max2 < cur2 -> output_L = i_L)) /\
+  (i_L < N <-> i_R < N) /\ N - i_L - 1 < k)
+)%Z.
+{
+clear.
+intros.
+destruct H as (((adj12 & i12 & out12 & outi1 & outi2 & i1N & kN & NN & cur12) & maxcur1) &  maxcur2).
+repeat split.
+1: assumption.
+all: try (intros ; exfalso ; by lia).
+1,3,4,5: try by lia.
+
+symmetry.
+(* the new left output is the current loop index i *)
+unfold output_L.
+(* the old right output is equal to the old left output *)
+rewrite -out12.
+(* that one in turn is equal to i if the current left max is below the current left sampled value *)
+apply outi1.
+(* and the left sampled value is indeed larger than the left max *)
+exact maxcur1.
+}
+
+symmetry.
+(* the old right output was equal to the old left *)
+rewrite -imax12.
+(* the old left is i if amax1 < a *)
+(* this doesn't make sense? the old left doesn't care about the current a *)
+apply amax1_i.
+exact case_l.
+
+      * iMod ec_zero as "ε0".
+        tp_store ; tp_pures ; tp_store ; tp_pures.
+        iApply ("IH" $! j with "[-HΦ]") ; [|by iFrame].
+        (* we need 0 credits for the IH since we just dealt with the case i=j, so i+1 <> j. *)
+        rewrite e ; case_bool_decide as Si_j ; try lia.
+        iFrame "rnm' ε0".
+
+assert
+(forall DB (adj : DB → DB → Prop) db1 db2 i1 i2 output1 output2 max1 max2 cur1 cur2 N k,
+  (((adj db1 db2 /\
+    i1 = i2 /\ output1 = output2 /\
+    (max1 < cur1 ->
+     output1 = i1) /\
+    (max2 < cur2 ->
+     output1 = i1) /\
+    i1 < N /\
+    k = N - i1 - 1 /\
+    N - i1 - 1 <= N /\ cur1 = cur2) /\
+   max1 < cur1) /\
+   ((max2 < cur2) -> False)) ->
+  (let i_R := i2 + 1 in
+  let i_L := i1 + 1 in
+  (output1 = output2 /\ adj db1 db2 /\
+   (i_L = i_R /\ i1 = output2) /\
+   (cur1 < cur1 -> i1 = i_L) /\
+   (max2 < cur2 -> i1 = i_L)) /\
+  (i_L < N <-> i_R < N) /\ N - i_L - 1 < k)
+)%Z.
+{
+clear.
+intros.
+destruct H as (((adj12 & i12 & out12 & outi1 & outi2 & i1N & kN & NN & cur12) & maxcur1) &  maxcur2).
+repeat split.
+1: assumption.
+all: try (intros ; exfalso ; by lia).
+all: try by lia.
+done.
+}
+clear H0.
+        iFrame. iPureIntro. repeat split. 1,2: intuition try lia.
+        subst. apply amax2_i. done.
+(*         intros Sj_N jj.
+           subst.
+   admit. *)
+
+      * iMod ec_zero as "ε0".
+        iApply ("IH" $! j with "[-HΦ]") ; iFrame.
+        rewrite e. case_bool_decide ; try lia. iFrame.
+        iFrame. iPureIntro. repeat split. 1,2: intuition try lia.
+        (* intros.
+           admit. *)
+        done.
+
+    + tp_bind (Laplace _ _ _).
+      wp_bind (Laplace _ _ _).
+      iMod ec_zero as "ε0".
+      iApply (wp_couple_laplace e1 e2 (e2 - e1)%Z 0%Z with "[$rnm' ε0]") => //.
+      {
+        eapply Zabs_ind ; intuition lia.
+      }
+      1: rewrite Rmult_0_l => //.
+      iNext ; iIntros (a) "rnm'" => /=.
+      wp_pures. tp_pures. tp_store ; tp_pures ; wp_store.
+      assert (amax1 < a → imax1 = i)%Z as amax1_i by admit.
+      assert (amax2 < a + (e2 - e1) → imax1 = i)%Z as amax2_i by admit.
+
+      tp_load ; wp_load ; tp_pures ; wp_pures.
+      destruct_decide (@bool_decide_reflect (amax1 < a)%Z _) as case_l.
+      all: destruct_decide (@bool_decide_reflect (amax2 < a + (e2 - e1))%Z _) as case_r.
+      all: tp_pures ; wp_pures.
+
+      * do 2 (tp_store ; tp_pures ; wp_store ; wp_pures).
+        iApply ("IH" $! j (i+1)%Z i with "[-HΦ]") ; iFrame.
+        repeat case_bool_decide ; try lia ; iFrame.
+        all: iPureIntro ; intuition lia.
+      * wp_store ; wp_pures ; wp_store ; wp_pures.
+        iApply ("IH" $! j (i+1)%Z with "[-HΦ]") ; iFrame.
+        iSplitL. 1: repeat case_bool_decide ; try lia ; iFrame.
+        all: iPureIntro ; intuition try lia.
+      * tp_store ; tp_pures ; tp_store ; tp_pures.
+        iApply ("IH" $! j (i+1)%Z with "[-HΦ]") ; iFrame.
+        iSplitL. 1: repeat case_bool_decide ; try lia ; iFrame.
+        all: iPureIntro ; intuition lia.
+        (* 1,2: admit. *)
+      * iApply ("IH" $! j (i+1)%Z with "[-HΦ]") ; iFrame.
+        repeat case_bool_decide ; try lia ; iFrame.
+        all: iPureIntro ; intuition lia.
+
+  Admitted.
 
   Lemma rnm_diffpriv_3 num den :
     (0 < IZR num / IZR den) →
@@ -150,30 +577,5 @@ Section rnm.
       Unshelve.
       all: f_equal.
     Qed.
-
-  Lemma rnm_diffpriv num den (evalQ : val) DB (dDB : Distance DB) (N : nat) :
-    (0 < IZR num / IZR den) →
-    (∀ i : Z, wp_sensitive (evalQ #i) 1 dDB dZ) →
-    wp_diffpriv (report_noisy_max num den evalQ #N) (IZR num / IZR den) dDB.
-  Proof with (tp_pures ; wp_pures).
-    intros εpos qi_sens.
-    iIntros (? c db db' db_adj Φ) "(rnm & ε) HΦ".
-    rewrite /report_noisy_max.
-    tp_pures.
-    tp_alloc as maxI2 "maxI2". tp_pures. tp_alloc as maxA2 "maxA2". do 5 tp_pure.
-    wp_pures. wp_alloc maxI1 as "maxI1". wp_alloc maxA1 as "maxA1". do 5 wp_pure.
-    rewrite -/(rnm_body num den evalQ dDB N db maxI1 maxA1).
-    rewrite -/(rnm_body num den evalQ dDB N db' maxI2 maxA2).
-
-    (* Todo generalize over the current iteration index (initially/now: 0) and come up with a better invariant / induction hypothesis. *)
-    iAssert (∃ i : Z, maxI1 ↦ #i ∗ maxI2 ↦ₛ #i ∗ ⌜ 0 <= i <= N ⌝%Z)%I with "[$maxI1 $maxI2]" as "maxI". 1: iPureIntro ; lia.
-    iAssert (∃ a : Z, maxA1 ↦ #a ∗ maxA2 ↦ₛ #a)%I with "[$maxA1 $maxA2]" as "maxA".
-    iRevert "maxA maxI".
-    iLöb as "IH".
-    iIntros "(% & maxA1 & maxA2) (% & maxI1 & maxI2 & %i_N)".
-    rewrite /rnm_body. tp_pures. 1: cbv ; auto. wp_pures. case_bool_decide ; tp_pures ; wp_pures.
-    - tp_load. wp_load. iApply "HΦ" => //.
-    - give_up.
-  Admitted.
 
 End rnm.
